intermediate/Veritas.Intermediate.Correctness.fst
@@ -18,7 +18,9 @@ open Veritas.Intermediate.TSLog
 open Veritas.Intermediate.Verify
 open Veritas.Intermediate.VerifierConfig
 
+module E=Veritas.EAC
 module I = Veritas.Interleave
+module SpecM = Veritas.Verifier.Merkle
 module IntL = Veritas.Intermediate.Logs
 module IntG = Veritas.Intermediate.Global
 module IntV = Veritas.Intermediate.Verify
@@ -168,15 +170,16 @@ let inductive_step_addm_caseB #vcfg
                               (sk: slot_id vcfg)
                               (sk_anc: slot_id vcfg{let ils_i = I.prefix ils i in
                                                     let vss_i = IntTS.thread_state_pre ils i in
-                                                    let sts = IntV.thread_store vss_i in                                                    
+                                                    let sts = IntV.thread_store vss_i in
                                                     induction_props ils_i /\
                                                     AddM_S? (I.index ils i) /\
                                                     inuse_slot sts sk /\ inuse_slot sts sk_anc /\
                                                     (let AddM_S s (k,v) s' = I.index ils i in
                                                      let k_anc = stored_key sts sk_anc in
                                                      let k' = stored_key sts s' in                                                      
-                                                     stored_key sts sk = k /\ k_anc <> k' /\ points_to sts sk_anc sk)})
+                                                     stored_key sts sk = k /\ k_anc = k' /\ points_to sts sk_anc sk)})
   : induction_props_or_hash_collision (I.prefix ils (i + 1)) = 
+  let tid = IntTS.thread_id_of ils i in
   let ilk = to_logk ils in  
   let ils_i = I.prefix ils i in
   let ilk_i = I.prefix ilk i in
@@ -200,31 +203,238 @@ let inductive_step_addm_caseB #vcfg
     assert(slot_points_to_is_merkle_points_to_local sts sk_anc sk d_anc);
     
     let mv_anc = to_merkle_value (stored_value sts sk_anc) in
-    assert(mv_points_to mv_anc d_anc k);
-    
-    admit()
+    // assert(mv_points_to mv_anc d_anc k);
 
-  (*
-  let tid = IntTS.thread_id_of ils i in                                          
-  
+    let k_anc = stored_key sts sk_anc in
+    // assert(SpecV.store_contains stk k_anc);
+    // assert(SpecV.stored_value stk k_anc = stored_value sts sk_anc);    
+    SpecTS.lemma_eac_value_is_stored_value ilk_i k_anc tid;    
+    lemma_mv_points_to_dir_correct ilk_i k_anc d_anc;
+    lemma_ismap_correct sts sk s';
+    // assert(s' = sk_anc);
+    None
+
+let inductive_step_addm_caseC #vcfg 
+                              (ils: IntTS.hash_verifiable_log vcfg)                               
+                              (i:I.seq_index ils)
+                              (sk: slot_id vcfg)
+                              (sk_anc: slot_id vcfg{let ils_i = I.prefix ils i in
+                                                    let vss_i = IntTS.thread_state_pre ils i in
+                                                    let sts = IntV.thread_store vss_i in
+                                                    induction_props ils_i /\
+                                                    AddM_S? (I.index ils i) /\
+                                                    inuse_slot sts sk /\ inuse_slot sts sk_anc /\
+                                                    (let AddM_S s (k,v) s' = I.index ils i in
+                                                     let k_anc = stored_key sts sk_anc in
+                                                     let k' = stored_key sts s' in                                                      
+                                                     stored_key sts sk = k /\ k_anc <> k' /\ points_to sts sk_anc sk)})
+  : induction_props_or_hash_collision (I.prefix ils (i + 1)) = 
+  let tid = IntTS.thread_id_of ils i in
+  let ilk = to_logk ils in  
+  let ils_i = I.prefix ils i in
+  let ilk_i = I.prefix ilk i in
+  let ils_i1 = I.prefix ils (i + 1) in
+  let ilk_i1 = I.prefix ilk (i + 1) in  
+  let vss_i = thread_state_pre ils i in
+  let vsk_i = SpecTS.thread_state_pre ilk i in
+  let vsk_i1 = SpecTS.thread_state_post ilk i in
+  let es = I.index ils i in
+  SpecTS.lemma_verifier_thread_state_extend ilk i;
+
   let ek = I.index ilk i in
 
   match es with
   | AddM_S s (k,v) s' ->
     let sts = IntV.thread_store vss_i in
-    let stk = SpecV.thread_store vsk_i in
+    let stk = SpecV.thread_store vsk_i in     
 
-    let sk = slot_of_key sts k in      
-  
-    admit()
-  *)
+    lemma_addm_props vss_i es;
+    let k' = stored_key sts s' in
+    let v' = to_merkle_value (stored_value sts s') in
+    let d = desc_dir k k' in
 
+    let d_anc = if points_to_dir sts sk_anc Left sk then Left else Right in
+    
+    (* we have the invariant that merkle value stored in sk_anc points to sk *)
+    assert(slot_points_to_is_merkle_points_to_local sts sk_anc sk d_anc);
+    
+    let mv_anc = to_merkle_value (stored_value sts sk_anc) in
+    // assert(mv_points_to mv_anc d_anc k);
+
+    let k_anc = stored_key sts sk_anc in
+    // assert(SpecV.store_contains stk k_anc);
+    // assert(SpecV.stored_value stk k_anc = stored_value sts sk_anc);    
+    SpecTS.lemma_eac_value_is_stored_value ilk_i k_anc tid;    
+    lemma_points_to_implies_proving_ancestor ilk_i k k_anc d_anc;
+    assert(k_anc = proving_ancestor ilk_i k);
+    
+    let aux () 
+      : Lemma (k' = Root \/ not (SpecTS.is_eac_state_init ilk_i k')) = 
+      if k' = Root then ()
+      else (
+        assert(SpecV.store_contains stk k');
+        SpecTS.lemma_instore_implies_eac_state_instore ilk_i k' tid
+      )
+    in
+    aux();
+    lemma_init_ancestor_ancestor_of_proving ilk_i k k';
+    SpecTS.lemma_eac_value_is_stored_value ilk_i k' tid;
+
+    let k2 = mv_pointed_key v' d in
+
+    lemma_proper_desc_depth_monotonic k k_anc;
+    assert(is_desc k2 k);
+    lemma_desc_depth_monotonic k2 k;
+    assert(is_desc k_anc k2);
+    lemma_desc_depth_monotonic k_anc k2;    
+    None
+
+let proving_ancestor #vcfg
+                     (ils: IntTS.hash_verifiable_log vcfg)
+                     (i:I.seq_index ils)
+                     (s:slot_id vcfg{let ils_i = I.prefix ils i in
+                                     let vss_i = thread_state_pre ils i in
+                                     let sts = IntV.thread_store vss_i in
+                                     induction_props ils_i /\ 
+                                     inuse_slot sts s /\ stored_key sts s <> Root}):
+  pk:merkle_key{let ils_i = I.prefix ils i in
+                 let vss_i = thread_state_pre ils i in
+                 let sts = IntV.thread_store vss_i in
+                 let k = stored_key sts s in
+                 let ilk = to_logk ils in
+                 let ilk_i = I.prefix ilk i in
+                 pk = SpecM.proving_ancestor ilk_i k} = 
+                   
+  admit()
+                 
+let inductive_step_addm_caseD #vcfg 
+                              (ils: IntTS.hash_verifiable_log vcfg)                               
+                              (i:I.seq_index ils)
+                              (sk: slot_id vcfg{let ils_i = I.prefix ils i in
+                                                let vss_i = IntTS.thread_state_pre ils i in
+                                                let sts = IntV.thread_store vss_i in
+                                                induction_props ils_i /\
+                                                AddM_S? (I.index ils i) /\
+                                                inuse_slot sts sk /\
+                                                add_method_of sts sk = BAdd /\
+                                                (let AddM_S s (k,v) s' = I.index ils i in
+                                                 let k' = stored_key sts s' in                                                 
+                                                 stored_key sts sk = k /\
+                                                 k' = proving_ancestor ils i sk)})
+  : induction_props_or_hash_collision (I.prefix ils (i + 1)) = 
+  let tid = IntTS.thread_id_of ils i in
+  let ilk = to_logk ils in  
+  let ils_i = I.prefix ils i in
+  let ilk_i = I.prefix ilk i in
+  let ils_i1 = I.prefix ils (i + 1) in
+  let ilk_i1 = I.prefix ilk (i + 1) in  
+  let vss_i = thread_state_pre ils i in
+  let vsk_i = SpecTS.thread_state_pre ilk i in
+  let vsk_i1 = SpecTS.thread_state_post ilk i in
+  let es = I.index ils i in
+  SpecTS.lemma_verifier_thread_state_extend ilk i;
+
+  let ek = I.index ilk i in
+
+  match es with
+  | AddM_S s (k,v) s' ->
+    let sts = IntV.thread_store vss_i in
+    let stk = SpecV.thread_store vsk_i in     
+
+    lemma_addm_props vss_i es;
+    let k' = stored_key sts s' in
+    let v' = to_merkle_value (stored_value sts s') in
+    let d = desc_dir k k' in
+
+    // assert (SpecV.store_contains stk k);
+    // assert (SpecV.add_method_of stk k = BAdd);
+    SpecTS.lemma_instore_implies_eac_state_instore ilk_i k tid;
+    SpecTS.lemma_eac_stored_addm ilk_i k;
+    // assert (E.add_method_of (SpecTS.eac_state_of_key ilk_i k) = SpecTS.stored_add_method ilk_i k);
+
+    let aux():
+      Lemma (SpecTS.stored_tid ilk_i k = tid) = 
+      let tid' = SpecTS.stored_tid ilk_i k in
+      if tid' = tid then ()
+      else
+        SpecTS.lemma_key_in_unique_store2 ilk_i k tid tid'
+    in
+    aux();
+    // assert (E.add_method_of (SpecTS.eac_state_of_key ilk_i k) = BAdd);
+    SpecM.lemma_proving_ancestor_blum_bit ilk_i k;
+
+    assert(SpecV.store_contains stk k');
+    SpecTS.lemma_eac_value_is_stored_value ilk_i k' tid;
+    assert(mv_evicted_to_blum v' d);
+    None
+
+let inductive_step_addm_caseE #vcfg 
+                              (ils: IntTS.hash_verifiable_log vcfg)                               
+                              (i:I.seq_index ils)
+                              (sk: slot_id vcfg{let ils_i = I.prefix ils i in
+                                                let vss_i = IntTS.thread_state_pre ils i in
+                                                let sts = IntV.thread_store vss_i in
+                                                induction_props ils_i /\
+                                                AddM_S? (I.index ils i) /\
+                                                inuse_slot sts sk /\
+                                                (let AddM_S s (k,v) s' = I.index ils i in
+                                                 let k' = stored_key sts s' in                                                 
+                                                 stored_key sts sk = k /\
+                                                 k' <> proving_ancestor ils i sk)})
+  : induction_props_or_hash_collision (I.prefix ils (i + 1)) = 
+  let tid = IntTS.thread_id_of ils i in
+  let ilk = to_logk ils in  
+  let ils_i = I.prefix ils i in
+  let ilk_i = I.prefix ilk i in
+  let ils_i1 = I.prefix ils (i + 1) in
+  let ilk_i1 = I.prefix ilk (i + 1) in  
+  let vss_i = thread_state_pre ils i in
+  let vsk_i = SpecTS.thread_state_pre ilk i in
+  let vsk_i1 = SpecTS.thread_state_post ilk i in
+  let es = I.index ils i in
+  SpecTS.lemma_verifier_thread_state_extend ilk i;
+
+  let ek = I.index ilk i in
+
+  match es with
+  | AddM_S s (k,v) s' ->
+    let sts = IntV.thread_store vss_i in
+    let stk = SpecV.thread_store vsk_i in     
+
+    lemma_addm_props vss_i es;
+    let k' = stored_key sts s' in
+    let v' = to_merkle_value (stored_value sts s') in
+    let d = desc_dir k k' in
+
+    let pk = proving_ancestor ils i sk in
+    let aux () 
+      : Lemma (k' = Root \/ not (SpecTS.is_eac_state_init ilk_i k')) = 
+      if k' = Root then ()
+      else (
+        assert(SpecV.store_contains stk k');
+        SpecTS.lemma_instore_implies_eac_state_instore ilk_i k' tid
+      )
+    in
+    aux();
+    lemma_init_ancestor_ancestor_of_proving ilk_i k k';
+    SpecTS.lemma_eac_value_is_stored_value ilk_i k' tid;
+
+    let k2 = mv_pointed_key v' d in
+
+    lemma_proper_desc_depth_monotonic k pk;
+    assert(is_desc k2 k);
+    lemma_desc_depth_monotonic k2 k;
+    assert(is_desc pk k2);
+    lemma_desc_depth_monotonic pk k2;    
+    None    
 
 let inductive_step_addm #vcfg 
                        (ils: IntTS.hash_verifiable_log vcfg) 
                        (i:I.seq_index ils{let ils_i = I.prefix ils i in
                                           induction_props ils_i /\
                                           AddM_S? (I.index ils i)}): induction_props_or_hash_collision (I.prefix ils (i + 1)) = 
+    admit()
+(*                                          
   let tid = IntTS.thread_id_of ils i in                                          
   let ilk = to_logk ils in  
   let ils_i = I.prefix ils i in
@@ -333,6 +543,7 @@ let inductive_step_addm #vcfg
     )
     else 
       inductive_step_addm_caseA ils i
+*)
 
 (* 
  * induction step: if all the induction properties hold for prefix of length i, 
