high/Veritas.Verifier.Merkle.fsti
@@ -99,3 +99,13 @@ val lemma_init_ancestor_ancestor_of_proving (itsl: TL.eac_log) (k:key) (k':key{i
                   let pk = proving_ancestor itsl k in
                   mv_points_to_some mv d /\
                   is_desc pk (mv_pointed_key mv d)))
+
+(* if a merkle value of key k points to a key kd in some direction d, then kd is a proper desc of 
+ * k in direction d *)
+val lemma_mv_points_to_dir_correct (itsl: TL.eac_log) (k:merkle_key) (d:bin_tree_dir):
+  Lemma (requires (let mv = eac_merkle_value itsl k in
+                   mv_points_to_some mv d))
+        (ensures (let mv = eac_merkle_value itsl k in
+                  let kd = mv_pointed_key mv d in
+                  is_proper_desc kd k /\
+                  d = desc_dir kd k))
